Make cview lemmas more usable

src/proof/algebra/cview.v
@@ -5,14 +5,12 @@ Section cview.
 
 Class cviewG Σ :=
   { #[global] cview_reversed_referenceG ::
-      reversed_reference.reversed_referenceG
-        (K:=KKey.t) (R:=KKey.t * types.UID.t) (V:=KObjectV.t)
-        (f:=obj_parent_ref) (g:=obj_ref) Σ; }.
+      @reversed_reference.reversed_referenceG
+        KKey.t _ _ (KKey.t * types.UID.t) _ _ KObjectV.t obj_parent_ref obj_ref Σ; }.
 
 Definition cviewΣ :=
-  reversed_reference.reversed_referenceΣ
-    (K:=KKey.t) (R:=KKey.t * types.UID.t) (V:=KObjectV.t)
-    (f:=obj_parent_ref) (g:=obj_ref).
+  @reversed_reference.reversed_referenceΣ
+    KKey.t _ _ (KKey.t * types.UID.t) _ _ KObjectV.t obj_parent_ref obj_ref.
 
 #[global]
 Instance subG_cviewG Σ :
@@ -20,162 +18,314 @@ Instance subG_cviewG Σ :
 Proof.
   intros Hsub.
   constructor.
-  exact (reversed_reference.subG_reversed_referenceG
-    (K:=KKey.t) (R:=KKey.t * types.UID.t) (V:=KObjectV.t)
-    (f:=obj_parent_ref) (g:=obj_ref)
-    Σ Hsub).
+  exact (@reversed_reference.subG_reversed_referenceG
+    KKey.t _ _ (KKey.t * types.UID.t) _ _ KObjectV.t obj_parent_ref obj_ref Σ Hsub).
 Qed.
 
 Context `{!cviewG Σ}.
 
 Definition own_auth γ (state: gmap KKey.t KObjectV.t)
     (used_reference: gset (KKey.t * types.UID.t)) : iProp Σ :=
-  reversed_reference.own_auth
-    (K:=KKey.t) (R:=KKey.t * types.UID.t) (V:=KObjectV.t)
-    (f:=obj_parent_ref) (g:=obj_ref)
+  @reversed_reference.own_auth
+    KKey.t _ _ (KKey.t * types.UID.t) _ _ KObjectV.t obj_parent_ref obj_ref Σ _
     γ state used_reference.
 
-Definition mk_frag (r: KKey.t * types.UID.t) (dq: dfrac) (ks: gset KKey.t) :=
-  reversed_reference.mk_frag
-    (K:=KKey.t) (R:=KKey.t * types.UID.t)
-    r dq ks.
+Definition mk_frag (key: KKey.t) (uid: types.UID.t) (dq: dfrac) (ks: gset KKey.t) :=
+  @reversed_reference.mk_frag
+    KKey.t _ _ (KKey.t * types.UID.t) _ _
+    (key, uid) dq ks.
 
-Definition own_frag γ (r: KKey.t * types.UID.t) dq (ks: gset KKey.t) : iProp Σ :=
-  reversed_reference.own_frag
-    (K:=KKey.t) (R:=KKey.t * types.UID.t) (V:=KObjectV.t)
-    (f:=obj_parent_ref) (g:=obj_ref)
-    γ r dq ks.
+Definition own_frag γ (key: KKey.t) (uid: types.UID.t) dq (ks: gset KKey.t) : iProp Σ :=
+  @reversed_reference.own_frag
+    KKey.t _ _ (KKey.t * types.UID.t) _ _ KObjectV.t obj_parent_ref obj_ref Σ _
+    γ (key, uid) dq ks.
 
 Global Instance own_auth_timeless γ state used_reference :
   Timeless (own_auth γ state used_reference).
 Proof. unfold own_auth. apply _. Qed.
 
-Global Instance own_frag_timeless γ r dq ks :
-  Timeless (own_frag γ r dq ks).
+Global Instance own_frag_timeless γ key uid dq ks :
+  Timeless (own_frag γ key uid dq ks).
 Proof. unfold own_frag. apply _. Qed.
 
-Lemma own_auth_frag_valid {γ state used_reference r dq ks}:
+Lemma own_auth_frag_valid {γ state used_reference pk puid dq ks}:
   own_auth γ state used_reference -∗
-  own_frag γ r dq ks -∗
-  ⌜ ks = dom (filter (λ '(_, v), obj_parent_ref v = Some r) state) ⌝ ∗
-  ⌜ r ∈ used_reference ⌝.
+  own_frag γ pk puid dq ks -∗
+  ⌜ ks = dom (filter (λ '(_, v), obj_parent_ref v = Some (pk, puid)) state) ⌝ ∗
+  ⌜ (pk, puid) ∈ used_reference ⌝.
 Proof.
   unfold own_auth, own_frag.
-  apply (reversed_reference.own_auth_frag_valid
-    (K:=KKey.t) (R:=KKey.t * types.UID.t) (V:=KObjectV.t)
-    (f:=obj_parent_ref) (g:=obj_ref)).
+  apply (@reversed_reference.own_auth_frag_valid
+    KKey.t _ _ (KKey.t * types.UID.t) _ _ KObjectV.t obj_parent_ref obj_ref Σ _
+    γ state used_reference (pk, puid) dq ks).
 Qed.
 
-Lemma create_child_vs {γ state used_reference r ks} k v cks:
+Lemma create_child_vs {γ state used_reference pk puid ks} k uid v cks:
+  uid = (KObjectV.objectmeta v).(ObjectMetaV.UID') →
   state !! k = None →
-  obj_parent_ref v = Some r →
-  obj_ref k v ≠ r →
-  dom (filter (λ '(_, v'), obj_parent_ref v' = Some (obj_ref k v)) state) = cks →
-  obj_ref k v ∉ used_reference →
+  obj_parent_ref v = Some (pk, puid) →
+  dom (filter (λ '(_, v'), obj_parent_ref v' = Some (k, uid)) state) = cks →
+  uid ∉ (set_map snd used_reference : gset types.UID.t) →
   own_auth γ state used_reference -∗
-  own_frag γ r 1 ks ==∗
-    own_auth γ (<[k := v]> state) (used_reference ∪ {[obj_ref k v]}) ∗
-    own_frag γ r 1 (ks ∪ {[k]}) ∗
-    own_frag γ (obj_ref k v) 1 cks.
+  own_frag γ pk puid 1 ks ==∗
+    own_auth γ (<[k := v]> state) (used_reference ∪ {[(k, uid)]}) ∗
+    own_frag γ pk puid 1 (ks ∪ {[k]}) ∗
+    own_frag γ k uid 1 cks.
 Proof.
-  intros Hak Hparent Hself Hcks Hfresh.
+  iIntros (Huid Hak Hparent Hcks Hfresh_uid) "Hauth Hfrag".
+  iAssert (⌜ (pk, puid) ∈ used_reference ⌝)%I as %Hparent_used.
+  { iPoseProof (own_auth_frag_valid with "[$Hauth] [$Hfrag]") as "[_ $]". }
+  subst uid.
+  assert (Hself : obj_ref k v ≠ (pk, puid)).
+  { intros Heq.
+    unfold obj_ref in Heq.
+    injection Heq as _ Huid_eq.
+    apply Hfresh_uid.
+    rewrite Huid_eq.
+    change (snd (pk, puid) ∈
+      (set_map (λ ku : KKey.t * types.UID.t, snd ku) used_reference : gset types.UID.t)).
+    eapply (elem_of_map_2 (λ ku : KKey.t * types.UID.t, snd ku)).
+    exact Hparent_used.
+  }
+  assert (Hpairfresh : obj_ref k v ∉ used_reference).
+  { intros Hin.
+    apply Hfresh_uid.
+    change (snd (obj_ref k v) ∈
+      (set_map (λ ku : KKey.t * types.UID.t, snd ku) used_reference : gset types.UID.t)).
+    eapply (elem_of_map_2 (λ ku : KKey.t * types.UID.t, snd ku)).
+    exact Hin.
+  }
   unfold own_auth, own_frag.
-  eapply (reversed_reference.create_child_vs
-    (K:=KKey.t) (R:=KKey.t * types.UID.t) (V:=KObjectV.t)
-    (f:=obj_parent_ref) (g:=obj_ref)); eauto.
+  iMod (@reversed_reference.create_reference_vs
+    KKey.t _ _ (KKey.t * types.UID.t) _ _ KObjectV.t obj_parent_ref obj_ref Σ _
+    γ state used_reference (pk, puid) ks k v cks
+    with "Hauth Hfrag") as "(Hauth & Hfrag & Hchildfrag)".
+  - exact Hak.
+  - exact Hparent.
+  - exact Hself.
+  - unfold obj_ref. exact Hcks.
+  - exact Hpairfresh.
+  - iModIntro. iFrame.
 Qed.
 
-Lemma adopt_orphan_vs {γ state used_reference r ks} k v v':
+Lemma create_child_vs2 {γ state used_reference pk puid ks} k uid v:
+  uid = (KObjectV.objectmeta v).(ObjectMetaV.UID') →
+  state !! k = None →
+  obj_parent_ref v = Some (pk, puid) →
+  map_Forall (λ k v,
+    no_speculative_parent_reference (KObjectV.objectmeta v) (set_map snd used_reference : gset types.UID.t)
+  ) state →
+  uid ∉ (set_map snd used_reference : gset types.UID.t) →
+  own_auth γ state used_reference -∗
+  own_frag γ pk puid 1 ks ==∗
+    own_auth γ (<[k := v]> state) (used_reference ∪ {[(k, uid)]}) ∗
+    own_frag γ pk puid 1 (ks ∪ {[k]}) ∗
+    own_frag γ k uid 1 ∅.
+Proof.
+  iIntros (Huid Hak Hparent Hvalid Hfresh_uid) "Hauth Hfrag".
+  subst uid.
+  assert (Hcks :
+    dom (filter (λ '(_, v'), obj_parent_ref v' = Some (k, obj_ref k v).2) state) = (∅ : gset KKey.t)).
+  { apply dom_empty_iff_L.
+    apply map_empty.
+    intros k'.
+    rewrite map_lookup_filter.
+    destruct (state !! k') as [obj|] eqn:Hlookup; [|done].
+    simpl.
+    case_decide as Hparent_to_new.
+    - exfalso.
+      pose proof (map_Forall_lookup_1 _ _ _ _ Hvalid Hlookup) as Hno_spec.
+      apply Hfresh_uid.
+      unfold no_speculative_parent_reference in Hno_spec.
+      unfold obj_parent_ref, meta_parent_ref in Hparent_to_new.
+      destruct ((KObjectV.objectmeta obj).(ObjectMetaV.OwnerReferences')) as [orefs|] eqn:Horefs; [|done].
+      destruct (list_find (λ oref : OwnerReferenceV.t, oref.(OwnerReferenceV.Controller') = Some true) orefs)
+        as [[idx oref]|] eqn:Hfind; [|done].
+      injection Hparent_to_new as _ Huid_eq.
+      rewrite <- Huid_eq.
+      eapply Hno_spec.
+      unfold meta_parent_ref_is, meta_parent_ref.
+      rewrite Horefs Hfind.
+      done.
+    - done.
+  }
+  iMod (create_child_vs k (obj_ref k v).2 v ∅ with "Hauth Hfrag")
+    as "(Hauth & Hfrag & Hchildfrag)".
+  - reflexivity.
+  - exact Hak.
+  - exact Hparent.
+  - rewrite /obj_ref /=. exact Hcks.
+  - exact Hfresh_uid.
+  - iModIntro. iFrame.
+Qed.
+
+Lemma adopt_orphan_vs {γ state used_reference pk puid ks} k v v':
   state !! k = Some v →
   obj_parent_ref v = None →
-  obj_parent_ref v' = Some r →
-  obj_ref k v = obj_ref k v' →
+  obj_parent_ref v' = Some (pk, puid) →
+  (KObjectV.objectmeta v).(ObjectMetaV.UID') = (KObjectV.objectmeta v').(ObjectMetaV.UID') →
   own_auth γ state used_reference -∗
-  own_frag γ r 1 ks ==∗
+  own_frag γ pk puid 1 ks ==∗
     own_auth γ (<[k := v']> state) used_reference ∗
-    own_frag γ r 1 (ks ∪ {[k]}).
+    own_frag γ pk puid 1 (ks ∪ {[k]}).
 Proof.
-  intros Hak Hnone Hparent Hg.
+  intros Hak Hnone Hparent Huid.
+  assert (Hg : obj_ref k v = obj_ref k v').
+  { unfold obj_ref.
+    simpl.
+    rewrite Huid.
+    done.
+  }
   unfold own_auth, own_frag.
-  eapply (reversed_reference.adopt_orphan_vs
-    (K:=KKey.t) (R:=KKey.t * types.UID.t) (V:=KObjectV.t)
-    (f:=obj_parent_ref) (g:=obj_ref)); eauto.
+  eapply (@reversed_reference.set_reference_vs
+    KKey.t _ _ (KKey.t * types.UID.t) _ _ KObjectV.t obj_parent_ref obj_ref Σ _
+    γ state used_reference (pk, puid) ks); eauto.
 Qed.
 
-Lemma release_child_vs {γ state used_reference r ks} k v v':
+Lemma release_child_vs {γ state used_reference pk puid ks} k v v':
   state !! k = Some v →
-  obj_parent_ref v = Some r →
+  obj_parent_ref v = Some (pk, puid) →
   obj_parent_ref v' = None →
-  obj_ref k v = obj_ref k v' →
+  (KObjectV.objectmeta v).(ObjectMetaV.UID') = (KObjectV.objectmeta v').(ObjectMetaV.UID') →
   own_auth γ state used_reference -∗
-  own_frag γ r 1 ks ==∗
+  own_frag γ pk puid 1 ks ==∗
     own_auth γ (<[k := v']> state) used_reference ∗
-    own_frag γ r 1 (ks ∖ {[k]}).
+    own_frag γ pk puid 1 (ks ∖ {[k]}).
 Proof.
   intros Hak Hparent Hnone Hg.
+  assert (Hobj_ref : obj_ref k v = obj_ref k v').
+  { unfold obj_ref.
+    simpl.
+    rewrite Hg.
+    done.
+  }
   unfold own_auth, own_frag.
-  eapply (reversed_reference.release_child_vs
-    (K:=KKey.t) (R:=KKey.t * types.UID.t) (V:=KObjectV.t)
-    (f:=obj_parent_ref) (g:=obj_ref)); eauto.
+  eapply (@reversed_reference.unset_reference_vs
+    KKey.t _ _ (KKey.t * types.UID.t) _ _ KObjectV.t obj_parent_ref obj_ref Σ _
+    γ state used_reference (pk, puid) ks); eauto.
 Qed.
 
-Lemma delete_child_vs {γ state used_reference r ks} k v:
+Lemma delete_child_vs {γ state used_reference pk puid ks} k v:
   state !! k = Some v →
-  obj_parent_ref v = Some r →
+  obj_parent_ref v = Some (pk, puid) →
   own_auth γ state used_reference -∗
-  own_frag γ r 1 ks ==∗
+  own_frag γ pk puid 1 ks ==∗
     own_auth γ (delete k state) used_reference ∗
-    own_frag γ r 1 (ks ∖ {[k]}).
+    own_frag γ pk puid 1 (ks ∖ {[k]}).
 Proof.
   intros Hak Hparent.
   unfold own_auth, own_frag.
-  eapply (reversed_reference.delete_child_vs
-    (K:=KKey.t) (R:=KKey.t * types.UID.t) (V:=KObjectV.t)
-    (f:=obj_parent_ref) (g:=obj_ref)); eauto.
+  eapply (@reversed_reference.delete_reference_vs
+    KKey.t _ _ (KKey.t * types.UID.t) _ _ KObjectV.t obj_parent_ref obj_ref Σ _
+    γ state used_reference (pk, puid) ks); eauto.
 Qed.
 
-Lemma delete_child_vs2 {γ state used_reference r ks} k:
+Lemma delete_child_vs2 {γ state used_reference pk puid ks} k:
   k ∈ ks →
   own_auth γ state used_reference -∗
-  own_frag γ r 1 ks ==∗
+  own_frag γ pk puid 1 ks ==∗
     own_auth γ (delete k state) used_reference ∗
-    own_frag γ r 1 (ks ∖ {[k]}).
+    own_frag γ pk puid 1 (ks ∖ {[k]}).
 Proof.
   intros Hk.
   unfold own_auth, own_frag.
-  eapply (reversed_reference.delete_child_vs2
-    (K:=KKey.t) (R:=KKey.t * types.UID.t) (V:=KObjectV.t)
-    (f:=obj_parent_ref) (g:=obj_ref)); eauto.
+  eapply (@reversed_reference.delete_reference_vs2
+    KKey.t _ _ (KKey.t * types.UID.t) _ _ KObjectV.t obj_parent_ref obj_ref Σ _
+    γ state used_reference (pk, puid) ks); eauto.
 Qed.
 
 Lemma simple_update_vs {γ state used_reference} k v v':
   state !! k = Some v →
   obj_parent_ref v = obj_parent_ref v' →
-  obj_ref k v = obj_ref k v' →
+  (KObjectV.objectmeta v).(ObjectMetaV.UID') = (KObjectV.objectmeta v').(ObjectMetaV.UID') →
   own_auth γ state used_reference ==∗
     own_auth γ (<[k := v']> state) used_reference.
 Proof.
   intros Hak Hparent Href.
+  assert (Hobj_ref : obj_ref k v = obj_ref k v').
+  { unfold obj_ref.
+    simpl.
+    rewrite Href.
+    done.
+  }
   unfold own_auth.
-  eapply (reversed_reference.simple_update_vs
-    (K:=KKey.t) (R:=KKey.t * types.UID.t) (V:=KObjectV.t)
-    (f:=obj_parent_ref) (g:=obj_ref)); eauto.
+  eapply (@reversed_reference.simple_update_vs
+    KKey.t _ _ (KKey.t * types.UID.t) _ _ KObjectV.t obj_parent_ref obj_ref Σ _
+    γ state used_reference); eauto.
 Qed.
 
-Lemma create_orphan_vs {γ state used_reference} k v cks:
+Lemma create_orphan_vs {γ state used_reference} k uid v cks:
+  uid = (KObjectV.objectmeta v).(ObjectMetaV.UID') →
   state !! k = None →
   obj_parent_ref v = None →
   dom (filter (λ '(_, v'), obj_parent_ref v' = Some (obj_ref k v)) state) = cks →
-  obj_ref k v ∉ used_reference →
+  uid ∉ (set_map snd used_reference : gset types.UID.t) →
   own_auth γ state used_reference ==∗
     own_auth γ (<[k := v]> state) (used_reference ∪ {[obj_ref k v]}) ∗
-    own_frag γ (obj_ref k v) 1 cks.
+    own_frag γ k uid 1 cks.
 Proof.
-  intros Hak Hnone Hcks Hfresh.
+  intros Huid Hak Hnone Hcks Hfresh.
+  subst uid.
+  assert (Hpairfresh : obj_ref k v ∉ used_reference).
+  { intros Hin.
+    apply Hfresh.
+    change (snd (obj_ref k v) ∈
+      (set_map (λ ku : KKey.t * types.UID.t, snd ku) used_reference : gset types.UID.t)).
+    eapply (elem_of_map_2 (λ ku : KKey.t * types.UID.t, snd ku)).
+    exact Hin.
+  }
   unfold own_auth, own_frag.
-  eapply (reversed_reference.create_orphan_vs
-    (K:=KKey.t) (R:=KKey.t * types.UID.t) (V:=KObjectV.t)
-    (f:=obj_parent_ref) (g:=obj_ref)); eauto.
+  eapply (@reversed_reference.simple_create_vs
+    KKey.t _ _ (KKey.t * types.UID.t) _ _ KObjectV.t obj_parent_ref obj_ref Σ _
+    γ state used_reference); eauto.
+Qed.
+
+Lemma create_orphan_vs2 {γ state used_reference} k uid v:
+  uid = (KObjectV.objectmeta v).(ObjectMetaV.UID') →
+  state !! k = None →
+  obj_parent_ref v = None →
+  map_Forall (λ k v,
+    no_speculative_parent_reference (KObjectV.objectmeta v) (set_map snd used_reference : gset types.UID.t)
+  ) state →
+  uid ∉ (set_map snd used_reference : gset types.UID.t) →
+  own_auth γ state used_reference ==∗
+    own_auth γ (<[k := v]> state) (used_reference ∪ {[obj_ref k v]}) ∗
+    own_frag γ k uid 1 ∅.
+Proof.
+  iIntros (Huid Hak Hnone Hvalid Hfresh) "Hauth".
+  subst uid.
+  assert (Hcks :
+    dom (filter (λ '(_, v'), obj_parent_ref v' = Some (obj_ref k v)) state) = (∅ : gset KKey.t)).
+  { apply dom_empty_iff_L.
+    apply map_empty.
+    intros k'.
+    rewrite map_lookup_filter.
+    destruct (state !! k') as [obj|] eqn:Hlookup; [|done].
+    simpl.
+    case_decide as Hparent_to_new.
+    - exfalso.
+      pose proof (map_Forall_lookup_1 _ _ _ _ Hvalid Hlookup) as Hno_spec.
+      apply Hfresh.
+      unfold no_speculative_parent_reference in Hno_spec.
+      unfold obj_parent_ref, meta_parent_ref in Hparent_to_new.
+      destruct ((KObjectV.objectmeta obj).(ObjectMetaV.OwnerReferences')) as [orefs|] eqn:Horefs; [|done].
+      destruct (list_find (λ oref : OwnerReferenceV.t, oref.(OwnerReferenceV.Controller') = Some true) orefs)
+        as [[idx oref]|] eqn:Hfind; [|done].
+      injection Hparent_to_new as _ Huid_eq.
+      rewrite <- Huid_eq.
+      eapply Hno_spec.
+      unfold meta_parent_ref_is, meta_parent_ref.
+      rewrite Horefs Hfind.
+      done.
+    - done.
+  }
+  iMod (create_orphan_vs k (obj_ref k v).2 v ∅ with "Hauth") as "(Hauth & Hfrag)".
+  - reflexivity.
+  - exact Hak.
+  - exact Hnone.
+  - exact Hcks.
+  - exact Hfresh.
+  - iModIntro. iFrame.
 Qed.
 
 Lemma delete_orphan_vs {γ state used_reference} k v:
@@ -186,9 +336,9 @@ Lemma delete_orphan_vs {γ state used_reference} k v:
 Proof.
   intros Hak Hnone.
   unfold own_auth.
-  eapply (reversed_reference.delete_orphan_vs
-    (K:=KKey.t) (R:=KKey.t * types.UID.t) (V:=KObjectV.t)
-    (f:=obj_parent_ref) (g:=obj_ref)); eauto.
+  eapply (@reversed_reference.simple_delete_vs
+    KKey.t _ _ (KKey.t * types.UID.t) _ _ KObjectV.t obj_parent_ref obj_ref Σ _
+    γ state used_reference); eauto.
 Qed.
 
 End cview.
